Implement ListSeq.Append without extra memory
and move the old version to the examples file

src/linear/ListSeq.dfy
@@ -63,6 +63,7 @@ class List<A> {
         assert exists i | n+1 <= i < |spine| :: spine[i] == x;
         var i: nat; i :| n+1 <= i < |spine| && spine[i] == x;
         assert spine[i].next == spine[n+1];
+        assert i+1 < |spine|;
         assert spine[i].next == spine[i+1];
         assert n <= i;
         assert n < i+1;
@@ -88,13 +89,56 @@ class List<A> {
     DistinctSpine();
   }
 
+  lemma NextNullImpliesLast(n: Node<A>)
+    requires Valid()
+    requires n in spine
+    requires n.next == null
+    ensures spine[|spine|-1] == n
+  {
+    if spine[|spine|-1] != n {
+      var i :| 0 <= i < |spine| && spine[i] == n;
+      assert i != |spine|-1;
+      assert spine[i].IsPrevOf(spine[i+1]);
+      assert spine[i+1] == null;
+      assert spine[i+1] != null;
+      assert false;
+    }
+  }
+
   static function ModelAux(xs: seq<Node<A>>): seq<A>
-    reads multiset(xs)
+    reads set x | x in xs :: x`data
   {
     if xs == [] then
       []
     else
+      assert xs[0] in xs;
+      assert forall x | x in xs[1..] :: x in xs;
       [xs[0].data] + ModelAux(xs[1..])
+  }
+
+  lemma ModelAuxCommutesConcat(xs: seq<Node<A>>, ys: seq<Node<A>>)
+    ensures ModelAux(xs + ys) == ModelAux(xs) + ModelAux(ys)
+  {
+    if xs == [] {
+      calc == {
+        ModelAux(xs + ys);
+        ModelAux([] + ys);
+        { assert [] + ys == ys; }
+        ModelAux(ys);
+        [] + ModelAux(ys);
+        ModelAux([]) + ModelAux(ys);
+      }
+    } else {
+      assert xs == [xs[0]] + xs[1..];
+      assert (xs + ys)[1..] == xs[1..] + ys;
+      calc == {
+        ModelAux(xs + ys);
+        [xs[0].data] + ModelAux(xs[1..] + ys);
+        { ModelAuxCommutesConcat(xs[1..], ys); }
+        [xs[0].data] + ModelAux(xs[1..]) + ModelAux(ys);
+        ModelAux(xs) + ModelAux(ys);
+      }
+    }
   }
 
   function Model(): seq<A>
@@ -107,9 +151,21 @@ class List<A> {
   constructor()
     ensures Valid()
     ensures Model() == []
+    ensures fresh(Repr())
   {
     head := null;
     spine := [];
+  }
+
+  method Copy(other: List<A>)
+    modifies this
+    requires other.Valid()
+    ensures Valid()
+    ensures Model() == other.Model()
+    ensures Repr() == other.Repr()
+  {
+    head := other.head;
+    spine := other.spine;
   }
 
   method Pop() returns (res: A)
@@ -156,26 +212,34 @@ class List<A> {
   }
 
   method Append(other: List<A>)
-    decreases Repr()
-    modifies this
+    modifies this, Repr()
     requires Valid()
     requires other.Valid()
-    // At first I didn't add the next precondition. In a language without
-    // verification like C maybe I would have forgotten about it, but the function
-    // doesn't work the way you expect it to if you don't keep this precondition
-    // in mind. This could have resulted in segmentation faults or buggy code.
-    // Another win for formal verification!
-    requires this != other
+    // needed so that we don't build a cyclic list:
+    requires Repr() !! other.Repr()
     ensures Valid()
     ensures Model() == old(Model()) + other.Model()
+    ensures Repr() == old(Repr()) + other.Repr()
   {
     if head == null {
       head := other.head;
       spine := other.spine;
     } else {
-      var x := Pop();
-      Append(other);
-      Push(x);
+      var last := head;
+      ghost var i := 0;
+      while last.next != null
+        decreases |spine| - i
+        invariant last != null
+        invariant 0 <= i < |spine|
+        invariant spine[i] == last
+      {
+        last := last.next;
+        i := i + 1;
+      }
+      NextNullImpliesLast(last);
+      last.next := other.head;
+      spine := spine + other.spine;
+      ModelAuxCommutesConcat(old(spine), other.spine);
     }
   }
 
