src/linear/ListSeq.Examples.dfy
@@ -1,0 +1,25 @@
+include "../../src/linear/ListSeq.dfy"
+
+// `Append` operation implemented externally.
+method Append<A>(self: List<A>, other: List<A>)
+  decreases self.Repr()
+  modifies self
+  requires self.Valid()
+  requires other.Valid()
+  // At first I didn't add the next precondition. In a language without
+  // verification like C maybe I would have forgotten about it, but the function
+  // doesn't work the way you expect it to if you don't keep this precondition
+  // in mind. This could have resulted in segmentation faults or buggy code.
+  // Another win for formal verification!
+  requires self != other
+  ensures self.Valid()
+  ensures self.Model() == old(self.Model()) + other.Model()
+{
+  if self.head == null {
+    self.Copy(other);
+  } else {
+    var x := self.Pop();
+    Append(self, other);
+    self.Push(x);
+  }
+}
